Additions to the Inductive Invariant and fixes for minor problems found in the process.
* Added RecordedPreparesHaveValidSenderID predicate for all honest
  replicas to be included in the Inductive Invariant.
* Added SentPreparesMatchRecordedPrePrepareIfHostInSameView predicate
  for all honest replicas to be included in the Inductive Invariant.
  This states that as long as an honest Replica is in a given View, it will
  send the same Prepare msg for a given Sequence ID and not change its mind.
* Moved IsReplica and IsClient predicates to cluster_config.s.dfy
* Fix for replica.i.dfy to check correctly that the recorded consensus
  messages from the network are sent from replicas.

cluster_config.s.dfy
@@ -1,4 +1,7 @@
+include "network.s.dfy"
+
 module ClusterConfig {
+  import opened HostIdentifiers
 
   datatype Constants = Constants(
     maxByzantineFaultyReplicas:nat,
@@ -39,6 +42,20 @@ module ClusterConfig {
       requires WF()
     {
       2 * F() + 1
+    }
+
+    predicate IsReplica(id:HostId)
+      requires WF()
+    {
+      && ValidHostId(id)
+      && 0 <= id < N()
+    }
+
+    predicate IsClient(id:HostId)
+      requires WF()
+    {
+      && ValidHostId(id)
+      && N() <= id < NumHosts()
     }
   }
 }
